theories/examples/allocator.v
@@ -1,3 +1,4 @@
+(* TODO: ressurect this file later *)
 From iris.base_logic Require Import invariants.
 From iris_ni.logrel Require Import types interp.
 From iris_ni.program_logic Require Import dwp heap_lang_lifting.
